NMake (and hence BigN): shiftr, shiftl now in the signature NSig (BACKPORT 12688)
 we export the "safe" version of these functions, working for all
 input and not only reasonably small shifting arg. The former
 "unsafe" shiftr and shiftl are now unsafe_shiftr and unsafe_shiftl.

git-svn-id: svn+ssh://scm.gforge.inria.fr/svn/coq/branches/v8.3@12738 85f007b7-540e-0410-9357-904b9bb8a0f7

theories/Numbers/Natural/BigN/NMake.v
@@ -389,21 +389,21 @@ Module Make (Import W0:CyclicType) <: NType.
 
  (** * Shift *)
 
- Definition safe_shiftr n x :=
+ Definition shiftr n x :=
    match compare n (Ndigits x) with
-   |  Lt => shiftr n x
+   |  Lt => unsafe_shiftr n x
    | _ => N0 w_0
    end.
 
- Theorem spec_safe_shiftr: forall n x,
-   [safe_shiftr n x] = [x] / 2 ^ [n].
+ Theorem spec_shiftr: forall n x,
+   [shiftr n x] = [x] / 2 ^ [n].
  Proof.
- intros n x; unfold safe_shiftr;
+ intros n x; unfold shiftr;
     generalize (spec_compare_aux n (Ndigits x)); case compare; intros H.
  apply trans_equal with (1 := spec_0 w0_spec).
  apply sym_equal; apply Zdiv_small; rewrite H.
  rewrite spec_Ndigits; exact (spec_digits x).
- rewrite <- spec_shiftr; auto with zarith.
+ rewrite <- spec_unsafe_shiftr; auto with zarith.
  apply trans_equal with (1 := spec_0 w0_spec).
  apply sym_equal; apply Zdiv_small.
  rewrite spec_Ndigits in H; case (spec_digits x); intros H1 H2.
@@ -412,22 +412,22 @@ Module Make (Import W0:CyclicType) <: NType.
  apply Zpower_le_monotone; auto with zarith.
  Qed.
 
- Definition safe_shiftl_aux_body cont n x :=
+ Definition shiftl_aux_body cont n x :=
    match compare n (head0 x)  with
       Gt => cont n (double_size x)
-   |  _ => shiftl n x
+   |  _ => unsafe_shiftl n x
    end.
 
- Theorem spec_safe_shift_aux_body: forall n p x cont,
+ Theorem spec_shiftl_aux_body: forall n p x cont,
        2^ Zpos p  <=  [head0 x]  ->
       (forall x, 2 ^ (Zpos p + 1) <= [head0 x]->
          [cont n x] = [x] * 2 ^ [n]) ->
-      [safe_shiftl_aux_body cont n x] = [x] * 2 ^ [n].
+      [shiftl_aux_body cont n x] = [x] * 2 ^ [n].
  Proof.
- intros n p x cont H1 H2; unfold safe_shiftl_aux_body.
+ intros n p x cont H1 H2; unfold shiftl_aux_body.
  generalize (spec_compare_aux n (head0 x)); case compare; intros H.
-  apply spec_shiftl; auto with zarith.
-  apply spec_shiftl; auto with zarith.
+  apply spec_unsafe_shiftl; auto with zarith.
+  apply spec_unsafe_shiftl; auto with zarith.
  rewrite H2.
  rewrite spec_double_size; auto.
  rewrite Zplus_comm; rewrite Zpower_exp; auto with zarith.
@@ -435,23 +435,23 @@ Module Make (Import W0:CyclicType) <: NType.
  rewrite Zpower_1_r; apply Zmult_le_compat_l; auto with zarith.
  Qed.
 
- Fixpoint safe_shiftl_aux p cont n x  {struct p} :=
-   safe_shiftl_aux_body
+ Fixpoint shiftl_aux p cont n x  {struct p} :=
+   shiftl_aux_body
        (fun n x => match p with
         | xH => cont n x
-        | xO p => safe_shiftl_aux p (safe_shiftl_aux p cont) n x
-        | xI p => safe_shiftl_aux p (safe_shiftl_aux p cont) n x
+        | xO p => shiftl_aux p (shiftl_aux p cont) n x
+        | xI p => shiftl_aux p (shiftl_aux p cont) n x
         end) n x.
 
- Theorem spec_safe_shift_aux: forall p q n x cont,
+ Theorem spec_shiftl_aux: forall p q n x cont,
     2 ^ (Zpos q) <= [head0 x] ->
       (forall x, 2 ^ (Zpos p + Zpos q) <= [head0 x] ->
          [cont n x] = [x] * 2 ^ [n]) ->
-      [safe_shiftl_aux p cont n x] = [x] * 2 ^ [n].
+      [shiftl_aux p cont n x] = [x] * 2 ^ [n].
  Proof.
- intros p; elim p; unfold safe_shiftl_aux; fold safe_shiftl_aux; clear p.
+ intros p; elim p; unfold shiftl_aux; fold shiftl_aux; clear p.
  intros p Hrec q n x cont H1 H2.
- apply spec_safe_shift_aux_body with (q); auto.
+ apply spec_shiftl_aux_body with (q); auto.
  intros x1 H3; apply Hrec with (q + 1)%positive; auto.
  intros x2 H4; apply Hrec with (p + q + 1)%positive; auto.
  rewrite <- Pplus_assoc.
@@ -462,7 +462,7 @@ Module Make (Import W0:CyclicType) <: NType.
    auto.
  repeat rewrite Zpos_plus_distr; ring.
  intros p Hrec q n x cont H1 H2.
- apply spec_safe_shift_aux_body with (q); auto.
+ apply spec_shiftl_aux_body with (q); auto.
  intros x1 H3; apply Hrec with (q); auto.
  apply Zle_trans with (2 := H3); auto with zarith.
  apply Zpower_le_monotone; auto with zarith.
@@ -473,34 +473,34 @@ Module Make (Import W0:CyclicType) <: NType.
    auto.
  repeat rewrite Zpos_plus_distr; ring.
  intros q n x cont H1 H2.
- apply spec_safe_shift_aux_body with (q); auto.
+ apply spec_shiftl_aux_body with (q); auto.
  rewrite Zplus_comm; auto.
  Qed.
 
- Definition safe_shiftl n x :=
-  safe_shiftl_aux_body
-   (safe_shiftl_aux_body
-    (safe_shiftl_aux (digits n) shiftl)) n x.
+ Definition shiftl n x :=
+  shiftl_aux_body
+   (shiftl_aux_body
+    (shiftl_aux (digits n) unsafe_shiftl)) n x.
 
- Theorem spec_safe_shift: forall n x,
-   [safe_shiftl n x] = [x] * 2 ^ [n].
+ Theorem spec_shiftl: forall n x,
+   [shiftl n x] = [x] * 2 ^ [n].
  Proof.
- intros n x; unfold safe_shiftl, safe_shiftl_aux_body.
+ intros n x; unfold shiftl, shiftl_aux_body.
  generalize (spec_compare_aux n (head0 x)); case compare; intros H.
-  apply spec_shiftl; auto with zarith.
-  apply spec_shiftl; auto with zarith.
+  apply spec_unsafe_shiftl; auto with zarith.
+  apply spec_unsafe_shiftl; auto with zarith.
  rewrite <- (spec_double_size x).
  generalize (spec_compare_aux n (head0 (double_size x))); case compare; intros H1.
-  apply spec_shiftl; auto with zarith.
-  apply spec_shiftl; auto with zarith.
+  apply spec_unsafe_shiftl; auto with zarith.
+  apply spec_unsafe_shiftl; auto with zarith.
  rewrite <- (spec_double_size (double_size x)).
- apply spec_safe_shift_aux with 1%positive.
+ apply spec_shiftl_aux with 1%positive.
  apply Zle_trans with (2 := spec_double_size_head0 (double_size x)).
  replace (2 ^ 1) with (2 * 1).
  apply Zmult_le_compat_l; auto with zarith.
  generalize (spec_double_size_head0_pos x); auto with zarith.
  rewrite Zpower_1_r; ring.
- intros x1 H2; apply spec_shiftl.
+ intros x1 H2; apply spec_unsafe_shiftl.
  apply Zle_trans with (2 := H2).
  apply Zle_trans with (2 ^ Zpos (digits n)); auto with zarith.
  case (spec_digits n); auto with zarith.
